Locally_Nameless_Lambda_Calculus/LN_Lambda_Strong_Normalization.thy
@@ -1,0 +1,350 @@
+theory LN_Lambda_Strong_Normalization
+  imports
+    LN_Lambda_Reduction
+    LN_Lambda_Typing
+begin
+
+text \<open>Strong normalization of the well-typed fragment, via Tait/Girard reducibility.
+
+  \<^bold>\<open>Status:\<close> this file currently contains only the definitions and the statements of every
+  lemma; all proofs are \<^theory_text>\<open>sorry\<close>, awaiting review before they are discharged.\<close>
+
+
+section \<open>Strong normalization predicate\<close>
+
+text \<open>\<open>SN t\<close> holds when every \<open>\<beta>\<close>-reduction sequence starting from \<open>t\<close> terminates. Rather than a
+  bespoke predicate we reuse the accessible part \<^const>\<open>Wellfounded.accp\<close> of one-step reduction;
+  \<open>SN\<close> is merely an abbreviation (no new constant), so all of \<^const>\<open>Wellfounded.accp\<close>'s library
+  (well-founded induction, etc.) is available directly.\<close>
+
+abbreviation SN :: "('\<tau>, '\<Sigma>, '\<V>) preterm \<Rightarrow> bool" where
+  "SN \<equiv> Wellfounded.accp beta_reduce\<inverse>\<inverse>"
+
+lemma SN_step: "SN t \<Longrightarrow> beta_reduce t u \<Longrightarrow> SN u"
+  by (meson accp.cases conversep_iff)
+
+lemma SN_AppD: "SN (App t u) \<Longrightarrow> SN t \<and> SN u"
+proof (induction "App t u" arbitrary: t u rule: accp_induct_rule)
+  case 1
+  then show ?case
+    unfolding conversep_iff
+    by (metis App_left App_right accpI)
+qed
+
+lemma SN_AbsD: "SN (Abs \<tau> t) \<Longrightarrow> SN t"
+proof (induction "Abs \<tau> t" arbitrary: \<tau> t rule: accp_induct_rule)
+  case 1
+  then show ?case
+    by (metis beta_reduce.Abs conversep_iff not_accp_down)
+qed
+
+lemma SN_ConstD: "SN (Const c \<tau>s ts) \<Longrightarrow> t \<in> set ts \<Longrightarrow> SN t"
+proof (induction "Const c \<tau>s ts" arbitrary: c \<tau>s ts t rule: accp_induct_rule)
+  case 1
+  note IH = "1.hyps"(2)
+  show ?case
+  proof (rule accpI)
+    fix t'
+    assume "beta_reduce\<inverse>\<inverse> t' t"
+    then have "beta_reduce t t'"
+      by simp
+    obtain i where "i < length ts" and "ts ! i = t"
+      using "1.prems" by (meson in_set_conv_nth)
+    then have "beta_reduce (Const c \<tau>s ts) (Const c \<tau>s (ts[i := t']))"
+      using \<open>beta_reduce t t'\<close> by (metis beta_reduce.Const)
+    moreover have "t' \<in> set (ts[i := t'])"
+      using \<open>i < length ts\<close> by (simp add: set_update_memI)
+    ultimately show "SN t'"
+      using IH by (metis conversep_iff)
+  qed
+qed
+
+lemma SN_subst_bound_FreeD: "SN (subst_bound 0 (Free x) t) \<Longrightarrow> SN t"
+  sorry
+
+text \<open>Bridge to the goal: if every element of a set is strongly normalizing, then the reversed
+  reduction relation is well-founded on that set.\<close>
+
+lemma wfp_on_beta_reduce_if_SN:
+  assumes "\<And>t. t \<in> A \<Longrightarrow> SN t"
+  shows "wfp_on A beta_reduce\<inverse>\<inverse>"
+proof -
+  have "Wellfounded.accp (\<lambda>x y. beta_reduce y x \<and> x \<in> A \<and> y \<in> A) y"
+    if "beta_reduce x y" and "y \<in> A" and "x \<in> A"
+    for x y
+    using assms(1)[OF \<open>y \<in> A\<close>, unfolded conversep_iff] that
+    by (smt (verit, ccfv_SIG) accpI accp_induct)
+
+  then show ?thesis
+  unfolding conversep_iff
+  unfolding wfp_on_iff_wfp[of A]
+  by (metis (no_types, lifting) accpI accp_wfpI)
+qed
+
+
+section \<open>Reducibility candidates\<close>
+
+text \<open>A term is \<^emph>\<open>neutral\<close> when it is not an abstraction; applying it to an argument creates no
+  redex at the root.\<close>
+
+definition neutral :: "('\<tau>, '\<Sigma>, '\<V>) preterm \<Rightarrow> bool" where
+  "neutral t \<longleftrightarrow> \<not> is_Abs t"
+
+text \<open>Reducibility \<open>Red \<tau> t\<close> is defined by recursion on the type \<open>\<tau>\<close>. We recurse on the underlying
+  \<^type>\<open>prety\<close> and lift the result to \<^type>\<open>ty\<close>. At a function type a term is reducible iff it is
+  strongly normalizing and sends reducible, locally closed arguments to reducible results; at any
+  other type reducibility is just strong normalization.\<close>
+
+fun Red_prety ::
+  "('\<V>\<^sub>t\<^sub>y, '\<Sigma>\<^sub>t\<^sub>y :: type_signature) prety \<Rightarrow>
+    (('\<V>\<^sub>t\<^sub>y, '\<Sigma>\<^sub>t\<^sub>y) ty, '\<Sigma>, '\<V>) preterm \<Rightarrow> bool" where
+  "Red_prety (PretyCtr \<kappa> [\<tau>\<^sub>1, \<tau>\<^sub>2]) t =
+    (if \<kappa> = fun_tyctr then
+       SN t \<and> (\<forall>u. locally_closed u \<longrightarrow> Red_prety \<tau>\<^sub>1 u \<longrightarrow> Red_prety \<tau>\<^sub>2 (App t u))
+     else SN t)" |
+  "Red_prety _ t = SN t"
+
+definition Red ::
+  "('\<V>\<^sub>t\<^sub>y, '\<Sigma>\<^sub>t\<^sub>y :: type_signature) ty \<Rightarrow> (('\<V>\<^sub>t\<^sub>y, '\<Sigma>\<^sub>t\<^sub>y) ty, '\<Sigma>, '\<V>) preterm \<Rightarrow> bool" where
+  "Red \<tau> t \<longleftrightarrow> Red_prety (Rep_ty \<tau>) t"
+
+
+lemma Red_TyFun:
+  "Red (TyFun \<tau>\<^sub>1 \<tau>\<^sub>2) t \<longleftrightarrow>
+     SN t \<and> (\<forall>u. locally_closed u \<longrightarrow> Red \<tau>\<^sub>1 u \<longrightarrow> Red \<tau>\<^sub>2 (App t u))"
+  unfolding Red_def TyCtr_def
+  by (simp add: Abs_ty_inverse wf_prety_PretyCtr_fun_tyctr)
+
+lemma size_ty_TyCtr:
+  assumes "length \<tau>s = arity \<kappa>"
+  shows "size_ty f\<^sub>1 f\<^sub>2 (TyCtr \<kappa> \<tau>s) = f\<^sub>2 \<kappa> + size_list (size_ty f\<^sub>1 f\<^sub>2) \<tau>s + Suc 0"
+proof -
+  have *: "Rep_ty (Abs_ty (PretyCtr \<kappa> (map Rep_ty \<tau>s))) = (PretyCtr \<kappa> (map Rep_ty \<tau>s))"
+  proof (rule Abs_ty_inverse[simplified])
+    show "wf_prety (PretyCtr \<kappa> (map Rep_ty \<tau>s))"
+      by (simp add: assms wf_prety_PretyCtr)
+  qed
+
+  then show ?thesis
+  unfolding TyCtr_def
+  unfolding size_ty.rep_eq
+  by (simp add: comp_def)
+qed
+
+lemma size_ty_TyFun: "size_ty f\<^sub>1 f\<^sub>2 (TyFun \<tau>\<^sub>1 \<tau>\<^sub>2) = f\<^sub>2 fun_tyctr + size_ty f\<^sub>1 f\<^sub>2 \<tau>\<^sub>1  + size_ty f\<^sub>1 f\<^sub>2 \<tau>\<^sub>2 + 3"
+  using size_ty_TyCtr[of "[\<tau>\<^sub>1, \<tau>\<^sub>2]" fun_tyctr, simplified]
+  by presburger
+
+function Red_ty ::
+  "('\<V>\<^sub>t\<^sub>y, '\<Sigma>\<^sub>t\<^sub>y :: type_signature) ty \<Rightarrow> (('\<V>\<^sub>t\<^sub>y, '\<Sigma>\<^sub>t\<^sub>y) ty, '\<Sigma>, '\<V>) preterm \<Rightarrow> bool" where
+  "Red_ty (TyFun \<tau>\<^sub>1 \<tau>\<^sub>2) t \<longleftrightarrow> (SN t \<and> (\<forall>u. locally_closed u \<longrightarrow> Red_ty \<tau>\<^sub>1 u \<longrightarrow> Red_ty \<tau>\<^sub>2 (App t u)))" |
+  "\<not> is_TyFun \<tau> \<Longrightarrow> Red_ty \<tau> t \<longleftrightarrow> SN t"
+proof -
+  \<comment> \<open>Pattern completeness\<close>
+  show "\<And>P x. (\<And>\<tau>\<^sub>1 \<tau>\<^sub>2 t. x = (TyFun \<tau>\<^sub>1 \<tau>\<^sub>2, t) \<Longrightarrow> P) \<Longrightarrow> (\<And>\<tau> t. \<not> is_TyFun \<tau> \<Longrightarrow> x = (\<tau>, t) \<Longrightarrow> P) \<Longrightarrow> P"
+    by (metis prod.exhaust)
+
+  \<comment> \<open>The remaining subgoals are pattern compatibility.\<close>
+qed auto
+termination
+proof (relation "measure (\<lambda>(\<tau>, t). size_ty (\<lambda>_. 0) (\<lambda>_. 0) \<tau>)")
+  show "wf (measure (\<lambda>(\<tau>, t). size_ty (\<lambda>_. 0) (\<lambda>_. 0) \<tau>))"
+    by simp
+next
+  fix \<tau>\<^sub>1 \<tau>\<^sub>2 t x
+  assume "locally_closed x"
+  then have "size_ty (\<lambda>_. 0) (\<lambda>_. 0) \<tau>\<^sub>1 < size_ty (\<lambda>_. 0) (\<lambda>_. 0) (TyFun \<tau>\<^sub>1 \<tau>\<^sub>2)"
+    unfolding size_ty_TyFun
+    by linarith
+  then show "((\<tau>\<^sub>1, x), TyFun \<tau>\<^sub>1 \<tau>\<^sub>2, t) \<in> measure (\<lambda>(\<tau>, t). size_ty (\<lambda>_. 0) (\<lambda>_. 0) \<tau>)"
+    by simp
+next
+  fix \<tau>\<^sub>1 \<tau>\<^sub>2 t x
+  assume "locally_closed x" and "Red_ty \<tau>\<^sub>1 x" and "Red_ty_dom (\<tau>\<^sub>1, x)"
+  then have "size_ty (\<lambda>_. 0) (\<lambda>_. 0) \<tau>\<^sub>2 < size_ty (\<lambda>_. 0) (\<lambda>_. 0) (TyFun \<tau>\<^sub>1 \<tau>\<^sub>2)"
+    unfolding size_ty_TyFun
+    by linarith
+  then show "((\<tau>\<^sub>2, App t x), TyFun \<tau>\<^sub>1 \<tau>\<^sub>2, t) \<in> measure (\<lambda>(\<tau>, t). size_ty (\<lambda>_. 0) (\<lambda>_. 0) \<tau>)"
+    by simp
+qed
+
+lemma "Red = Red_ty"
+proof (intro ext)
+  fix \<tau> t
+  show "Red \<tau> t = Red_ty \<tau> t"
+  proof (induction \<tau> t rule: Red_ty.induct)
+    case (1 \<tau>\<^sub>1 \<tau>\<^sub>2 t)
+    then show ?case
+      by (simp add: Red_TyFun)
+  next
+    case (2 \<tau> t)
+    then show ?case
+    proof (induction \<tau>)
+      case (TyVar x)
+      then show ?case
+        by (simp add: Red_def TyVar_def Abs_ty_inverse wf_prety.PretyVar)
+    next
+      case (TyCtr \<kappa> \<tau>s)
+      have "\<kappa> \<noteq> fun_tyctr"
+        using TyCtr.prems TyCtr.hyps
+        by (metis (no_types, lifting) arity\<^sub>_tyctr_simps(2) length_0_conv length_Suc_conv numerals(2))
+
+      then have "Red (TyCtr \<kappa> \<tau>s) t = SN t"
+        using wf_prety_PretyCtr[OF \<open>length \<tau>s = arity \<kappa>\<close>]
+        by (cases "(PretyCtr \<kappa> (map Rep_ty \<tau>s), t)" rule: Red_prety.cases)
+          (simp_all add: Red_def TyCtr_def Abs_ty_inverse[simplified])
+      also have "SN t = Red_ty (TyCtr \<kappa> \<tau>s) t"
+        using TyCtr.prems by simp
+      finally show ?case .
+    qed
+  qed
+qed
+
+section \<open>Reducibility candidate properties (CR1--CR3)\<close>
+
+lemma CR1: "Red \<tau> t \<Longrightarrow> SN t"
+proof -
+  assume a1: "Red \<tau> t"
+  have "\<forall>t. All ((\<lambda>p. SN p \<or> \<not> Red t p)::(('a, 'b) ty, 'c, 'd) preterm \<Rightarrow> _)"
+    by (smt (verit) Red_def Red_prety.elims(2))
+  then show ?thesis
+    using a1 by blast
+qed
+
+lemma CR2:
+  assumes "Red \<tau> t" and "beta_reduce t t'"
+  shows "Red \<tau> t'"
+proof -
+  have "Red_prety p a \<Longrightarrow> beta_reduce a b \<Longrightarrow> Red_prety p b" for p a b
+  proof (induction p a arbitrary: b rule: Red_prety.induct)
+    case (1 \<kappa> \<tau>\<^sub>1 \<tau>\<^sub>2 a)
+    show ?case
+    proof (cases "\<kappa> = fun_tyctr")
+      case True
+      have "SN a"
+        using "1.prems"(1) True by simp
+      then have "SN b"
+        using "1.prems"(2) SN_step by blast
+      moreover have "Red_prety \<tau>\<^sub>2 (App b u)"
+        if u: "locally_closed u" "Red_prety \<tau>\<^sub>1 u" for u
+      proof -
+        have "Red_prety \<tau>\<^sub>2 (App a u)"
+          using "1.prems"(1) True u by simp
+        moreover have "beta_reduce (App a u) (App b u)"
+          using "1.prems"(2) by (rule beta_reduce.App_left)
+        ultimately show ?thesis
+          using "1.IH"(2)[OF True u(1) u(2)] by blast
+      qed
+      ultimately show ?thesis
+        using True by simp
+    next
+      case False
+      have "SN a"
+        using "1.prems"(1) False by simp
+      then have "SN b"
+        using "1.prems"(2) SN_step by blast
+      then show ?thesis
+        using False by simp
+    qed
+  qed (auto intro: SN_step)
+  then show ?thesis
+    using assms unfolding Red_def by blast
+qed
+
+lemma CR3:
+  "neutral t \<Longrightarrow> locally_closed t \<Longrightarrow> (\<And>t'. beta_reduce t t' \<Longrightarrow> Red \<tau> t') \<Longrightarrow> Red \<tau> t"
+  sorry
+
+text \<open>In particular, free variables are reducible at every type (they are neutral and normal).\<close>
+
+lemma Red_Free: "Red \<tau> (Free x)"
+  sorry
+
+
+section \<open>Reducibility of abstractions and constants\<close>
+
+lemma Red_Abs:
+  assumes inf_vars: "infinite (UNIV :: '\<V> set)"
+  assumes "locally_closed (Abs \<tau>\<^sub>1 t)"
+  assumes "\<And>u. locally_closed u \<Longrightarrow> Red \<tau>\<^sub>1 u \<Longrightarrow> Red \<tau>\<^sub>2 (subst_bound 0 u t)"
+  shows "Red (TyFun \<tau>\<^sub>1 \<tau>\<^sub>2) (Abs \<tau>\<^sub>1 t)"
+  sorry
+
+lemma Red_Const:
+  assumes "locally_closed (Const c \<tau>s ts)"
+  assumes "\<forall>t \<in> set ts. SN t"
+  shows "Red \<tau> (Const c \<tau>s ts)"
+  sorry
+
+
+section \<open>Parallel substitution of free variables\<close>
+
+text \<open>Simultaneous substitution of the free (named) variables. Contrary to \<^const>\<open>subst_bound\<close>,
+  this descends into the parameters of a constant, which may contain free variables.\<close>
+
+fun msubst ::
+  "('\<V> \<Rightarrow> ('\<tau>, '\<Sigma>, '\<V>) preterm) \<Rightarrow> ('\<tau>, '\<Sigma>, '\<V>) preterm \<Rightarrow> ('\<tau>, '\<Sigma>, '\<V>) preterm" where
+  "msubst \<theta> (Const c \<tau>s ts) = Const c \<tau>s (map (msubst \<theta>) ts)" |
+  "msubst \<theta> (Free x) = \<theta> x" |
+  "msubst \<theta> (Bound n) = Bound n" |
+  "msubst \<theta> (App t\<^sub>1 t\<^sub>2) = App (msubst \<theta> t\<^sub>1) (msubst \<theta> t\<^sub>2)" |
+  "msubst \<theta> (Abs \<tau> t) = Abs \<tau> (msubst \<theta> t)"
+
+lemma msubst_Free: "msubst Free t = t"
+  by (induction t) (simp_all add: map_idI)
+
+lemma msubst_cong:
+  "(\<And>z. z \<in> free_vars t \<Longrightarrow> \<theta> z = \<theta>' z) \<Longrightarrow> msubst \<theta> t = msubst \<theta>' t"
+  by (induction t) (auto cong: map_cong)
+
+lemma locally_closed_msubst:
+  "(\<And>y. locally_closed (\<theta> y)) \<Longrightarrow> locally_closed t \<Longrightarrow> locally_closed (msubst \<theta> t)"
+  sorry
+
+text \<open>Opening a fresh variable and then substituting it equals substituting into the opened body
+  (the key commutation lemma for the abstraction case of the fundamental theorem).\<close>
+
+lemma msubst_subst_bound_Free:
+  assumes inf_vars: "infinite (UNIV :: '\<V> set)"
+  assumes "x \<notin> free_vars t"
+  assumes "\<And>y. locally_closed (\<theta> y)"
+  shows "msubst (\<theta>(x := u)) (subst_bound n (Free x) t) = subst_bound n u (msubst \<theta> t)"
+  sorry
+
+
+section \<open>Fundamental theorem and strong normalization\<close>
+
+text \<open>Every well-typed term is reducible under any reducible, locally closed substitution of its
+  free variables.\<close>
+
+lemma fundamental:
+  assumes inf_vars: "infinite (UNIV :: '\<V> set)"
+  assumes "has_type \<C> \<F> t \<tau>"
+  assumes "\<And>x. locally_closed (\<theta> x)"
+  assumes "\<And>x. Red (\<F> x) (\<theta> x)"
+  shows "Red \<tau> (msubst \<theta> t)"
+  sorry
+
+lemma SN_if_has_type:
+  assumes inf_vars: "infinite (UNIV :: '\<V> set)"
+  assumes ht: "has_type \<C> \<F> t \<tau>"
+  shows "SN t"
+proof -
+  have "Red \<tau> (msubst Free t)"
+  proof (rule fundamental[OF inf_vars ht])
+    show "\<And>x. locally_closed (Free x)"
+      by (rule locally_closed.Free)
+  next
+    show "\<And>x. Red (\<F> x) (Free x)"
+      by (rule Red_Free)
+  qed
+  then show "SN t"
+    by (metis CR1 msubst_Free)
+qed
+
+proposition strong_normalization_of_typed_terms:
+  assumes inf_vars: "infinite (UNIV :: '\<V> set)"
+  shows "wfp_on {t. \<exists>\<C> \<F> \<tau>. has_type \<C> \<F> t \<tau>} beta_reduce\<inverse>\<inverse>"
+  by (rule wfp_on_beta_reduce_if_SN) (auto intro: SN_if_has_type[OF inf_vars])
+
+end
